Ensured that the function which calculates a node in the trellis in the fast way in the absence of the previous row behaves correctly in the zeroth time-step. Ensured that the slow version of the viterbi trellis code is evaluable using EVAL_TAC. Fixed the slow version of the function which computes a trellis node so that the origin is NONE if we are at time step 0. Wrote test to test the equivalence of the slow and fast trellis calculation functions for small values of s and t, and wrote a test to test that they return the correct result at time step 0.

convolutional_codesScript.sml
@@ -1131,9 +1131,12 @@ Definition viterbi_trellis_row_def:
       GENLIST (λn. viterbi_trellis_node m bs n (SUC t) previous_row) m.num_states
 End
 
+(* -------------------------------------------------------------------------- *)
+(* Calculate a node in the trellis for the fast version when the previous row *)
+(* is not available (by calculating all prior rows of the trellis)            *)
+(* -------------------------------------------------------------------------- *)
 Definition viterbi_trellis_node_no_prev_data:
-  viterbi_trellis_node_no_prev_data m bs s t =
-  viterbi_trellis_node m bs s t (viterbi_trellis_row m bs (t - 1))
+  viterbi_trellis_node_no_prev_data m bs s t = EL s (viterbi_trellis_row m bs t)
 End
 
 (* -------------------------------------------------------------------------- *)
@@ -1144,10 +1147,10 @@ End
 (* recursively dependent on each other.                                       *)
 (* -------------------------------------------------------------------------- *)
 Definition viterbi_trellis_slow:
-  get_num_errors_calculate_slow m bs (SUC 0) r = (if (r.origin = 0) then N0 else INFINITY) ∧
-  (get_num_errors_calculate_slow m bs (SUC (SUC t)) r =
-   (get_num_errors_calculate_slow m bs (SUC t) (best_origin_slow m bs (SUC t) r.origin)) + N (hamming_distance (m.transition_fn r).output (relevant_input m bs (SUC (SUC t))))
-  ) ∧ 
+  get_num_errors_calculate_slow m bs 0 r = (if ((m.transition_fn r).destination = 0) then N0 else INFINITY) ∧
+  (get_num_errors_calculate_slow m bs (SUC t) r =
+   (get_num_errors_calculate_slow m bs t (best_origin_slow m bs t r.origin)) + N (hamming_distance (m.transition_fn r).output (relevant_input m bs (SUC t)))
+   ) ∧ 
   (get_better_origin_slow m bs t r1 r2 =
    if (get_num_errors_calculate_slow m bs t r1) < (get_num_errors_calculate_slow m bs t r2) then r1 else r2) ∧
   (best_origin_slow m bs t s =
@@ -1206,23 +1209,37 @@ Definition viterbi_trellis_node_slow_def:
     best_origin_local = best_origin_slow m bs t s;
   in
     <| num_errors := get_num_errors_calculate_slow m bs t best_origin_local;
-       prev_state := SOME best_origin_local.origin; |>
-End
+       prev_state := if (t = 0) then NONE else SOME best_origin_local.origin; |>
+End  
 
+(* -------------------------------------------------------------------------- *)
+(* Test equivalance of slow version of trellis calculation with fast version  *)
+(* for some small values of s and t, through evaluation.                      *)
+(* -------------------------------------------------------------------------- *)
 Theorem viterbi_trellis_node_slow_test:
-  let
-    s = 0;
-    t = 2
-  in
-    viterbi_trellis_node_slow example_state_machine test_path s t = ARB ∧
-    viterbi_trellis_node_no_prev_data example_state_machine test_path s t = ARB
+  ∀s t.
+  s < 4 ∧ t ≤ 3 ⇒
+  viterbi_trellis_node_slow example_state_machine test_path s t = viterbi_trellis_node_no_prev_data example_state_machine test_path s t
 Proof
-  EVAL_TAC
-  >> qspecl_then [‘0’, ‘transition_origin 0 F’, ‘example_state_machine’, ‘test_path ’] assume_tac (cj 2 get_num_errors_calculate_slow_def)
-  >> gvs[]
-  >> gvs[example_state_machine_def, test_path_def]
+  rpt strip_tac
+  >> sg ‘(s = 0 ∨ s = 1 ∨ s = 2 ∨ s = 3) ∧ (t = 0 ∨ t = 1 ∨ t = 2 ∨ t = 3)’ >> gvs[]
   >> EVAL_TAC
-  >> pop_assum (fn th => gvs[th])
+QED
+
+(* -------------------------------------------------------------------------- *)
+(* Be extra careful with the special case at time step zero, and test to      *)
+(* ensure that it has the expected value, not just the same value as the      *)
+(* other implementation.                                                      *)
+(* -------------------------------------------------------------------------- *)
+Theorem viterbi_trellis_node_slow_time_step_zero_test:
+  ∀s.
+  s < 4 ⇒
+  viterbi_trellis_node_slow example_state_machine test_path s 0 =
+                     <| num_errors := if s = 0 then N0 else INFINITY; prev_state := NONE|>
+Proof
+  rpt strip_tac
+  >> sg ‘(s = 0 ∨ s = 1 ∨ s = 2 ∨ s = 3)’ >> gvs[]
+  >> EVAL_TAC
 QED
 
 
